\documentclass{article}
\usepackage{akwon}
\setlength{\parindent}{0pt}
\title{Homework 2 feedback}
\author{}
\date{18/20}
\begin{document}
\maketitle
\begin{enumerate}
	\item For (b), there was an arithmetic error. $\frac{\pi}{3} \cos(\pi/3) = \pi/6$, not $1/6$.
	\item Good!
	\item (1/2) The problem was quite clear about how you should compute the derivative from the limit definition. It goes as follows:
		\begin{align*}
			\frac{\sqrt[3]{x+h} - \sqrt[3]{x}}{h} \cdot \frac{\sqrt[3]{x+h}^{2} + \sqrt[3]{x+h} \sqrt[3]{x} + \sqrt[3]{x}^{2}}{\sqrt[3]{x+h}^{2} + \sqrt[3]{x+h} \sqrt[3]{x} + \sqrt[3]{x}^{2}} &= \frac{\sqrt[3]{x+h}^{3} - \sqrt[3]{x}^{3}}{h \cdot (\sqrt[3]{x+h}^{2} + \sqrt[3]{x+h} \sqrt[3]{x} + \sqrt[3]{x}^{2})}\\
			&= \frac{1}{\sqrt[3]{x+h}^{2} + \sqrt[3]{x+h} \sqrt[3]{x} + \sqrt[3]{x}^{2}},
		\end{align*}
		and taking $h \to 0$ we find that the limit is equal to $\frac{1}{3 \sqrt[3]{x^{2}}} = \frac{1}{3} x^{-2/3}$.
	\item Good!
	\item Good!
	\item Good!
	\item Good!
	\item (1/2) Why is the slope 2? More detail is needed.\\
		Here's is summary of the solution: the equation of the tangent line passing through an arbitrary point $(a, a^{2})$ is 
		\[
			(y - a^{2}) = (2a) (x - a) \Leftrightarrow y = 2ax - a^{2}.
		\]
		Thus, in order for this line to pass through the point $(0, -1)$, we need $a^{2} = 1$, hence $a = \pm 1$ and the two equations are given by $y = 2x -1$, $y = -2x - 1$.
\end{enumerate}
\end{document}
